wip

code/bignum/Hacl.Impl.Exponentiation.fst
@@ -168,9 +168,9 @@ let lexp_pow_in_place #a_t len ctx_len k ctx acc b =
     k.lsqr ctx acc acc)
 
 
-///////////////////////////////////////////////////////////////////
-//// the precomputed table and constant-time access to its elements
-//////////////////////////////////////////////////////////////////
+///////////////////////////////////////////////////////////////////////
+//// the precomputed table and constant-time access to its elements ///
+///////////////////////////////////////////////////////////////////////
 
 inline_for_extraction noextract
 val precomp_table_inv:
@@ -179,7 +179,7 @@ val precomp_table_inv:
   -> ctx_len:size_t
   -> k:concrete_ops a_t len ctx_len
   -> a:LSeq.lseq (uint_t a_t SEC) (v len)
-  -> table_len:size_t{1 < v table_len /\ v table_len * v len <= max_size_t}
+  -> table_len:size_t{v table_len * v len <= max_size_t}
   -> table:LSeq.lseq (uint_t a_t SEC) (v table_len * v len)
   -> j:nat{j < v table_len} ->
   Type0
@@ -188,8 +188,154 @@ let precomp_table_inv #a_t len ctx_len k a table_len table j =
   Math.Lemmas.lemma_mult_le_right (v len) (j + 1) (v table_len);
   let bj = LSeq.sub table (j * v len) (v len) in
   k.to.linv bj /\ k.to.linv a /\
- (let table_s = SE.precomp_table k.to.concr_ops (k.to.refl a) (v table_len) in
-  k.to.refl bj == LSeq.index table_s j)
+  k.to.refl bj == SE.pow k.to.concr_ops (k.to.refl a) j
+
+
+inline_for_extraction noextract
+val lprecomp_table_mul:
+    #a_t:inttype_a
+  -> len:size_t{v len > 0}
+  -> ctx_len:size_t
+  -> k:concrete_ops a_t len ctx_len
+  -> ctx:lbuffer (uint_t a_t SEC) ctx_len
+  -> a:lbuffer (uint_t a_t SEC) len
+  -> i:size_t
+  -> ti:lbuffer (uint_t a_t SEC) len
+  -> res:lbuffer (uint_t a_t SEC) len ->
+  Stack unit
+  (requires fun h ->
+    live h a /\ live h ti /\ live h ctx /\ live h res /\
+    disjoint a ti /\ disjoint a ctx /\ disjoint a res /\
+    disjoint ti ctx /\ disjoint ti res /\ disjoint ctx res /\
+    k.to.linv (as_seq h a) /\ k.to.linv_ctx (as_seq h ctx) /\
+    k.to.linv (as_seq h ti) /\
+    k.to.refl (as_seq h ti) == SE.pow k.to.concr_ops (k.to.refl (as_seq h a)) (v i + 1))
+  (ensures  fun h0 _ h1 -> modifies (loc res) h0 h1 /\
+    k.to.linv (as_seq h1 res) /\
+    k.to.refl (as_seq h1 res) == SE.pow k.to.concr_ops (k.to.refl (as_seq h0 a)) (v i + 2))
+
+let lprecomp_table_mul #a_t len ctx_len k ctx a i ti res =
+  let h0 = ST.get () in
+  k.lmul ctx a ti res;
+  let h1 = ST.get () in
+  assert (k.to.refl (as_seq h1 res) == k.to.concr_ops.SE.mul (k.to.refl (as_seq h0 a)) (k.to.refl (as_seq h0 ti)));
+  SE.pow_unfold k.to.concr_ops (k.to.refl (as_seq h0 a)) (v i + 2)
+
+
+#push-options "--z3rlimit 150"
+inline_for_extraction noextract
+val precomp_table_inv_lemma_j:
+    #a_t:inttype_a
+  -> len:size_t{v len > 0}
+  -> ctx_len:size_t
+  -> k:concrete_ops a_t len ctx_len
+  -> a:LSeq.lseq (uint_t a_t SEC) (v len)
+  -> table_len:size_t{v table_len * v len <= max_size_t}
+  -> table1:LSeq.lseq (uint_t a_t SEC) (v table_len * v len)
+  -> table2:LSeq.lseq (uint_t a_t SEC) (v table_len * v len)
+  -> i:nat{i <= v table_len}
+  -> j:nat{j < i} -> Lemma
+  (requires
+    LSeq.sub table1 0 (i * v len) == LSeq.sub table2 0 (i * v len) /\
+    precomp_table_inv len ctx_len k a table_len table1 j)
+  (ensures
+    precomp_table_inv len ctx_len k a table_len table2 j)
+
+let precomp_table_inv_lemma_j #a_t len ctx_len k a table_len table1 table2 i j =
+  assert (precomp_table_inv len ctx_len k a table_len table1 j);
+  Math.Lemmas.lemma_mult_le_right (v len) (j + 1) (v table_len);
+  let bj1 = LSeq.sub table1 (j * v len) (v len) in
+  let bj2 = LSeq.sub table2 (j * v len) (v len) in
+
+  let aux (l:nat{l < v len}) : Lemma (LSeq.index bj1 l == LSeq.index bj2 l) =
+    Seq.lemma_index_slice table1 (j * v len) (j * v len + v len) l;
+    assert (LSeq.index bj1 l == LSeq.index table1 (j * v len + l));
+    Seq.lemma_index_slice table2 (j * v len) (j * v len + v len) l;
+    assert (LSeq.index bj2 l == LSeq.index table2 (j * v len + l));
+    Seq.lemma_index_slice table1 0 (i * v len) (j * v len + l);
+    Seq.lemma_index_slice table2 0 (i * v len) (j * v len + l);
+    assert (LSeq.index table1 (j * v len + l) == LSeq.index table2 (j * v len + l));
+    assert (LSeq.index bj1 l == LSeq.index bj2 l) in
+
+  Classical.forall_intro aux;
+  LSeq.eq_intro bj1 bj2;
+  assert (precomp_table_inv len ctx_len k a table_len table2 j)
+#pop-options
+
+
+inline_for_extraction noextract
+val precomp_table_inv_lemma:
+    #a_t:inttype_a
+  -> len:size_t{v len > 0}
+  -> ctx_len:size_t
+  -> k:concrete_ops a_t len ctx_len
+  -> a:LSeq.lseq (uint_t a_t SEC) (v len)
+  -> table_len:size_t{v table_len * v len <= max_size_t}
+  -> table1:LSeq.lseq (uint_t a_t SEC) (v table_len * v len)
+  -> table2:LSeq.lseq (uint_t a_t SEC) (v table_len * v len)
+  -> i:nat{i <= v table_len} -> Lemma
+  (requires
+    LSeq.sub table1 0 (i * v len) == LSeq.sub table2 0 (i * v len) /\
+    (forall (j:nat{j < i}). precomp_table_inv len ctx_len k a table_len table1 j))
+  (ensures
+    (forall (j:nat{j < i}). precomp_table_inv len ctx_len k a table_len table2 j))
+
+let precomp_table_inv_lemma #a_t len ctx_len k a table_len table1 table2 i =
+  let aux (j:nat{j < i}) : Lemma (precomp_table_inv len ctx_len k a table_len table2 j) =
+    assert (precomp_table_inv len ctx_len k a table_len table1 j);
+    precomp_table_inv_lemma_j #a_t len ctx_len k a table_len table1 table2 i j;
+    assert (precomp_table_inv len ctx_len k a table_len table2 j) in
+
+  Classical.forall_intro aux
+
+
+inline_for_extraction noextract
+val lprecomp_table_f:
+    #a_t:inttype_a
+  -> len:size_t{v len > 0}
+  -> ctx_len:size_t
+  -> k:concrete_ops a_t len ctx_len
+  -> ctx:lbuffer (uint_t a_t SEC) ctx_len
+  -> a:lbuffer (uint_t a_t SEC) len
+  -> table_len:size_t{1 < v table_len /\ v table_len * v len <= max_size_t}
+  -> i:size_t{v i < v table_len - 2}
+  -> table:lbuffer (uint_t a_t SEC) (table_len *! len) ->
+  Stack unit
+  (requires fun h ->
+    live h a /\ live h table /\ live h ctx /\
+    disjoint a table /\ disjoint ctx table /\ disjoint a ctx /\
+    k.to.linv (as_seq h a) /\ k.to.linv_ctx (as_seq h ctx) /\
+    (forall (j:nat{j <= v i + 1}).
+      precomp_table_inv len ctx_len k (as_seq h a) table_len (as_seq h table) j))
+  (ensures  fun h0 _ h1 -> modifies (loc table) h0 h1 /\
+    (forall (j:nat{j <= v i + 2}).
+      precomp_table_inv len ctx_len k (as_seq h0 a) table_len (as_seq h1 table) j))
+
+#push-options "--z3rlimit 300"
+let lprecomp_table_f #a_t len ctx_len k ctx a table_len i table =
+  Math.Lemmas.lemma_mult_le_right (v len) (v i + 2) (v table_len);
+  Math.Lemmas.lemma_mult_le_right (v len) (v i + 3) (v table_len);
+  assert (v ((i +! 1ul) *! len) == (v i + 1) * v len);
+  assert (v ((i +! 2ul) *! len) == (v i + 2) * v len);
+
+  let h0 = ST.get () in
+  assert (precomp_table_inv len ctx_len k (as_seq h0 a) table_len (as_seq h0 table) (v i + 1));
+  let t1 = sub table ((i +! 1ul) *! len) len in
+  let t2 = sub table ((i +! 2ul) *! len) len in
+  lprecomp_table_mul len ctx_len k ctx a i t1 t2;
+  let h1 = ST.get () in
+  B.modifies_buffer_elim (B.gsub #(uint_t a_t SEC) table 0ul ((i +! 2ul) *! len)) (loc t2) h0 h1;
+  assert (precomp_table_inv len ctx_len k (as_seq h0 a) table_len (as_seq h1 table) (v i + 2));
+  LSeq.eq_intro
+    (LSeq.sub (as_seq h0 table) 0 ((v i + 2) * v len))
+    (LSeq.sub (as_seq h1 table) 0 ((v i + 2) * v len));
+
+  assert (forall (j:nat{j <= v i + 1}).
+    precomp_table_inv len ctx_len k (as_seq h0 a) table_len (as_seq h0 table) j);
+  precomp_table_inv_lemma len ctx_len k (as_seq h0 a) table_len (as_seq h0 table) (as_seq h1 table) (v i + 2);
+  assert (forall (j:nat{j <= v i + 1}).
+    precomp_table_inv len ctx_len k (as_seq h0 a) table_len (as_seq h1 table) j)
+#pop-options
 
 
 inline_for_extraction noextract
@@ -210,8 +356,8 @@ val lprecomp_table:
     k.to.linv (as_seq h (gsub table 0ul len)) /\
     k.to.refl (as_seq h (gsub table 0ul len)) == k.to.concr_ops.SE.one ())
   (ensures  fun h0 _ h1 -> modifies (loc table) h0 h1 /\
-    (forall (j:nat{j < v table_len}).
-      precomp_table_inv #a_t len ctx_len k (as_seq h0 a) table_len (as_seq h0 table) j))
+    (forall (j:nat{j < v table_len}).{:pattern precomp_table_inv len ctx_len k (as_seq h1 a) table_len (as_seq h1 table) j}
+      precomp_table_inv len ctx_len k (as_seq h1 a) table_len (as_seq h1 table) j))
 
 let lprecomp_table #a_t len ctx_len k ctx a table_len table =
   let t0 = sub table 0ul len in
@@ -219,13 +365,14 @@ let lprecomp_table #a_t len ctx_len k ctx a table_len table =
   let h0 = ST.get () in
   copy t1 a;
   let h1 = ST.get () in
-  assert (k.to.refl (as_seq h1 (gsub table 0ul len)) == k.to.concr_ops.SE.one ());
-  assert (k.to.refl (as_seq h1 (gsub table len len)) == k.to.refl (as_seq h0 a));
+  //B.modifies_buffer_elim (B.gsub #(uint_t a_t SEC) table 0ul len) (loc t1) h0 h1;
+  LSeq.eq_intro (as_seq h0 t0) (as_seq h1 t0);
   assert (k.to.linv (as_seq h1 t0) /\ k.to.linv (as_seq h1 t1));
-  //assert (precomp_table_inv len ctx_len k (as_seq h0 a) table_len (as_seq h1 table) 0);
-  //assert (precomp_table_inv len ctx_len k (as_seq h0 a) table_len (as_seq h1 table) 1);
+  SE.pow_eq0 k.to.concr_ops (k.to.refl (as_seq h0 a));
+  SE.pow_eq1 k.to.concr_ops (k.to.refl (as_seq h0 a));
+  assert (precomp_table_inv len ctx_len k (as_seq h0 a) table_len (as_seq h1 table) 0);
+  assert (precomp_table_inv len ctx_len k (as_seq h0 a) table_len (as_seq h1 table) 1);
 
-  admit();
   [@ inline_let]
   let inv h (i:nat{i <= v table_len - 2}) =
     modifies (loc table) h1 h /\
@@ -235,9 +382,7 @@ let lprecomp_table #a_t len ctx_len k ctx a table_len table =
 
   Lib.Loops.for 0ul (table_len -! 2ul) inv
   (fun j ->
-    let t1 = sub table ((j +! 1ul) *! len) len in
-    let t2 = sub table ((j +! 2ul) *! len) len in
-    k.lmul ctx t1 a t2)
+    lprecomp_table_f #a_t len ctx_len k ctx a table_len j table)
 
 //////////////////////////////////////////////////////////
 
@@ -303,7 +448,69 @@ let bn_get_bits_c #b_t bLen bBits b l =
   BN.bn_get_bits bLen b i l
 
 
-(*)
+inline_for_extraction noextract
+let lprecomp_get_st
+  (a_t:inttype_a)
+  (len:size_t{v len > 0})
+  (ctx_len:size_t)
+  (k:concrete_ops a_t len ctx_len) =
+    a:lbuffer (uint_t a_t SEC) len
+  -> table_len:size_t{1 < v table_len /\ v table_len * v len <= max_size_t}
+  -> table:lbuffer (uint_t a_t SEC) (table_len *! len)
+  -> bits_l:uint_t a_t SEC{v bits_l < v table_len}
+  -> tmp:lbuffer (uint_t a_t SEC) len ->
+  Stack unit
+  (requires fun h ->
+    live h a /\ live h table /\ live h tmp /\
+    disjoint a table /\ disjoint a tmp /\ disjoint table tmp /\
+    k.to.linv (as_seq h a) /\
+    (forall (j:nat{j < v table_len}).
+      precomp_table_inv len ctx_len k (as_seq h a) table_len (as_seq h table) j))
+  (ensures  fun h0 _ h1 -> modifies (loc tmp) h0 h1 /\
+    k.to.linv (as_seq h1 tmp) /\
+    k.to.refl (as_seq h1 tmp) == SE.pow k.to.concr_ops (k.to.refl (as_seq h0 a)) (v bits_l))
+
+
+inline_for_extraction noextract
+val lprecomp_get_vartime:
+     #a_t:inttype_a
+  -> len:size_t{v len > 0}
+  -> ctx_len:size_t
+  -> k:concrete_ops a_t len ctx_len ->
+  lprecomp_get_st a_t len ctx_len k
+
+let lprecomp_get_vartime #a_t len ctx_len k a table_len table bits_l tmp =
+  let bits_l32 = Lib.RawIntTypes.(size_from_UInt32 (u32_to_UInt32 (to_u32 bits_l))) in
+  assert (v bits_l32 == v bits_l /\ v bits_l < v table_len);
+  Math.Lemmas.lemma_mult_le_right (v len) (v bits_l + 1) (v table_len);
+  assert (v (bits_l32 *! len) == v bits_l32 * v len);
+
+  let h0 = ST.get () in
+  let a_bits_l = sub table (bits_l32 *! len) len in
+  let h1 = ST.get () in
+  assert (precomp_table_inv len ctx_len k (as_seq h0 a) table_len (as_seq h0 table) (v bits_l));
+  assert (k.to.refl (as_seq h1 a_bits_l) == SE.pow k.to.concr_ops (k.to.refl (as_seq h0 a)) (v bits_l));
+  copy tmp a_bits_l
+
+
+inline_for_extraction noextract
+val lprecomp_get_consttime:
+     #a_t:inttype_a
+  -> len:size_t{v len > 0}
+  -> ctx_len:size_t
+  -> k:concrete_ops a_t len ctx_len ->
+  lprecomp_get_st a_t len ctx_len k
+
+let lprecomp_get_consttime #a_t len ctx_len k a table_len table bits_l tmp =
+  Math.Lemmas.lemma_mult_le_right (v len) (v bits_l + 1) (v table_len);
+  let h0 = ST.get () in
+  PT.table_select_consttime len table_len table bits_l tmp;
+  let h1 = ST.get () in
+  assert (as_seq h1 tmp == LSeq.sub (as_seq h0 table) (v bits_l * v len) (v len));
+  assert (precomp_table_inv len ctx_len k (as_seq h0 a) table_len (as_seq h0 table) (v bits_l));
+  assert (k.to.refl (as_seq h1 tmp) == SE.pow k.to.concr_ops (k.to.refl (as_seq h0 a)) (v bits_l))
+
+
 inline_for_extraction noextract
 let lmul_acc_pow_a_bits_l_st
   (a_t:inttype_a)
@@ -334,7 +541,7 @@ let lmul_acc_pow_a_bits_l_st
     k.to.linv (as_seq h1 acc) /\
     k.to.refl (as_seq h1 acc) ==
     SE.mul_acc_pow_a_bits_l #k.to.t_spec k.to.concr_ops (k.to.refl (as_seq h0 a))
-      (v bBits) (BD.bn_v h0 b) (v l) (v table_len) () (k.to.refl (as_seq h0 acc)))
+      (v bBits) (BD.bn_v h0 b) (v l) (v i) (k.to.refl (as_seq h0 acc)))
 
 
 inline_for_extraction noextract
@@ -386,7 +593,7 @@ let lexp_fw_f_st
   (ensures  fun h0 _ h1 -> modifies (loc acc) h0 h1 /\
     k.to.linv (as_seq h1 acc) /\
     k.to.refl (as_seq h1 acc) ==
-    S.exp_fw_f #k.to.a_spec k.to.concr_ops (k.to.refl (as_seq h0 a))
+    SE.exp_fw_f #k.to.t_spec k.to.concr_ops (k.to.refl (as_seq h0 a))
       (v bBits) (BD.bn_v h0 b) (v l) (v i) (k.to.refl (as_seq h0 acc)))
 
 
@@ -431,7 +638,7 @@ let lexp_fw_loop_st
       precomp_table_inv len ctx_len k (as_seq h a) table_len (as_seq h table) j))
   (ensures  fun h0 _ h1 -> modifies (loc acc) h0 h1 /\ k.to.linv (as_seq h1 acc) /\
     k.to.refl (as_seq h1 acc) ==
-    Loops.repeati (v bBits / v l) (S.exp_fw_f k.to.concr_ops (k.to.refl (as_seq h0 a))
+    Loops.repeati (v bBits / v l) (SE.exp_fw_f k.to.concr_ops (k.to.refl (as_seq h0 a))
       (v bBits) (BD.bn_v h0 b) (v l)) (k.to.refl (as_seq h0 acc)))
 
 
@@ -448,9 +655,9 @@ let lexp_fw_loop #a_t len ctx_len k lprecomp_get ctx a bLen bBits b l table_len 
   let h0 = ST.get () in
 
   [@ inline_let]
-  let refl1 i : GTot k.to.a_spec = k.to.refl (as_seq h0 acc) in
+  let refl1 i : GTot k.to.t_spec = k.to.refl (as_seq h0 acc) in
   [@inline_let]
-  let spec (h:mem) = S.exp_fw_f k.to.concr_ops (k.to.refl (as_seq h0 a))
+  let spec (h:mem) = SE.exp_fw_f k.to.concr_ops (k.to.refl (as_seq h0 a))
     (v bBits) (BD.bn_v h0 b) (v l) in
 
   [@inline_let]
@@ -496,7 +703,7 @@ let lexp_fw_acc0_st
   (ensures  fun h0 _ h1 -> modifies (loc acc) h0 h1 /\
     k.to.linv (as_seq h1 acc) /\
     k.to.refl (as_seq h1 acc) ==
-    S.exp_fw_acc0 k.to.concr_ops (k.to.refl (as_seq h0 a)) (v bBits) (BD.bn_v h0 b) (v l))
+    SE.exp_fw_acc0 k.to.concr_ops (k.to.refl (as_seq h0 a)) (v bBits) (BD.bn_v h0 b) (v l))
 
 
 inline_for_extraction noextract
@@ -537,13 +744,13 @@ let lexp_fw_gen_st
     disjoint acc ctx /\ disjoint acc table /\ disjoint ctx table /\
     BD.bn_v h b < pow2 (v bBits) /\
     k.to.linv_ctx (as_seq h ctx) /\ k.to.linv (as_seq h a) /\
-    k.to.linv (as_seq h acc) /\ k.to.refl (as_seq h acc) == k.to.concr_ops.S.one /\
+    k.to.linv (as_seq h acc) /\ k.to.refl (as_seq h acc) == k.to.concr_ops.SE.one () /\
     (forall (j:nat{j < v table_len}).
       precomp_table_inv len ctx_len k (as_seq h a) table_len (as_seq h table) j))
   (ensures  fun h0 _ h1 -> modifies (loc acc) h0 h1 /\
     k.to.linv (as_seq h1 acc) /\
     k.to.refl (as_seq h1 acc) ==
-    S.exp_fw k.to.concr_ops (k.to.refl (as_seq h0 a)) (v bBits) (BD.bn_v h0 b) (v l))
+    SE.exp_fw k.to.concr_ops (k.to.refl (as_seq h0 a)) (v bBits) (BD.bn_v h0 b) (v l))
 
 
 inline_for_extraction noextract
@@ -583,7 +790,7 @@ let lexp_fw_gen #a_t len ctx_len k lprecomp_get ctx a bLen bBits b acc l =
   let table = create (table_len *! len) (uint #a_t #SEC 0) in
   update_sub table 0ul len acc;
   let h = ST.get () in
-  assert (k.to.refl (as_seq h (gsub table 0ul len)) == k.to.concr_ops.S.one);
+  assert (k.to.refl (as_seq h (gsub table 0ul len)) == k.to.concr_ops.SE.one ());
   lprecomp_table #a_t len ctx_len k ctx a table_len table;
   lexp_fw_gen_ #a_t len ctx_len k lprecomp_get ctx a bLen bBits b l table_len table acc;
   pop_frame ()
